Cslib.lean
@@ -148,7 +148,6 @@ public import Cslib.Languages.LambdaCalculus.LocallyNameless.Untyped.Properties
 public import Cslib.Languages.LambdaCalculus.LocallyNameless.Untyped.StandardReduction
 public import Cslib.Languages.LambdaCalculus.LocallyNameless.Untyped.StrongNorm
 public import Cslib.Languages.LambdaCalculus.LocallyNameless.Untyped.Abstract
-public import Cslib.Languages.LambdaCalculus.LocallyNameless.Untyped.TakahashiSupport
 public import Cslib.Languages.LambdaCalculus.LocallyNameless.Untyped.Takahashi
 public import Cslib.Languages.LambdaCalculus.LocallyNameless.Untyped.ParEta
 public import Cslib.Languages.LambdaCalculus.Named.Untyped.Basic
